nets rework

basic_topology/T5_nets.lean
@@ -1,3 +1,4 @@
+
 import basic_topology.T0_topology
 import basic_topology.T3_sequences
 
@@ -8,113 +9,75 @@ set_option linter.style.multiGoal false
 
 universe u v
 
-variable {X Y : Type*}
+variable {X Y D: Type*}
+
 
 /-- A relation between `X` and `Y` is a binary predicate `X → Y → Prop`. -/
-def Relation (X : Type u) (Y : Type v) : Type (max u v) :=
+def Relation (X: Type u) (Y: Type v): Type (max u v) :=
   X → Y → Prop
 
 /-- An endorelation is a relation on a single set. -/
-def Endorelation (X : Type u) : Type u :=
+def Endorelation (X: Type u): Type u :=
   Relation X X
 
 /-- A preorder is a reflexive and transitive relation. -/
-structure preorder (X : Type u) (R : Relation X X) : Prop where
-  reflexive : ∀ x, R x x
-  transitive : ∀ x y z, (R x y ∧ R y z) → R x z
+structure preorder (R: Endorelation X): Prop where
+  reflexive: ∀ x, R x x
+  transitive: ∀ x y z, R x y → R y z → R x z
 
 /-- A directed set is a preorder where any two elements have an upper bound. -/
-structure directed_set (X : Type u) (R : Relation X X) : Prop where
-  reflexive : ∀ x, R x x
-  transitive : ∀ x y z, (R x y ∧ R y z) → R x z
-  upperbound : ∀ x y, ∃ z, R x z ∧ R y z
-
-/-- A net in `X` is a function from a directed set into `X`. -/
-structure net (X : Type u) where
-  (D : Type v)
-  (R : Relation D D)
-  [is_directed : directed_set D R]
-  (a : D → X)
-def f_net {X Y : Type*} (f : X → Y) (n : net X) : net Y :=
-  { D := n.D,
-    R := n.R,
-    is_directed := n.is_directed,
-    a := fun i => f (n.a i) }
+structure directed (R: Endorelation X): Prop extends preorder R where
+  upperbound: ∀ x y, ∃ z, R x z ∧ R y z
 
 /-- A net `n` converges to `x` with respect to the topology `𝒯`
 iff every open neighborhood of `x` eventually contains all later terms of the net. -/
-def net_converges {X : Type u} (T: Set (Set X)) (n : net X) (x : X) : Prop :=
-  ∀ U : Set X, (U ∈ T) → (x ∈ U) →
-    ∃ i₀ : n.D, ∀ j : n.D, n.R i₀ j → n.a j ∈ U
-def f_net_converges
-  {X Y : Type*}
-  (TY : Set (Set Y))
-  (f : X → Y)
-  (n : net X)
-  (y : Y) : Prop :=
-  net_converges TY (f_net f n) y
+def net_converges (T: Set (Set X)) (R: Endorelation D) (n: D → X) (x: X): Prop :=
+  ∀ U ∈ Nbhds T x, ∃ i₀, ∀ i, R i₀ i → n i ∈ U
+
 /--
 The neighborhood net of a point `x` is a net constructed from the directed set of
 neighborhoods of `x`, where the direction is given by reverse subset inclusion.
 For each neighborhood `V`, a point `a(V)` is chosen from `V` using the axiom of choice.
 -/
-noncomputable def neighborhood_net {X : Type u} (TX: Set (Set X)) (hTX : IsTopology TX) (x : X) : net X where
-  D := { V : Set X // V ∈ Nbhds TX x }
-  R := fun U V => V.1 ⊆ U.1
-  is_directed := {
-    reflexive := fun U => Set.Subset.refl U.1,
-    transitive := fun _ _ _ h => Set.Subset.trans h.2 h.1,
-    upperbound := fun U V => by
-      have h_inter_nhds : U.1 ∩ V.1 ∈ Nbhds TX x := by
-        obtain ⟨O_U, hO_U_open, hx_in_OU, hOU_sub_U⟩ := U.2
-        obtain ⟨O_V, hO_V_open, hx_in_OV, hOV_sub_V⟩ := V.2
-        use O_U ∩ O_V
-        exact ⟨binary_inter_open hTX hO_U_open hO_V_open, ⟨hx_in_OU, hx_in_OV⟩, Set.inter_subset_inter hOU_sub_U hOV_sub_V⟩
-      use ⟨U.1 ∩ V.1, h_inter_nhds⟩
-      exact ⟨Set.inter_subset_left, Set.inter_subset_right⟩
-  }
-  a := fun V => Classical.choose (Set.nonempty_of_mem (neighborhood_mem V.2))
 
-/-- The neighborhood net of a point `x` converges to `x`. -/
-theorem neighborhood_net_converges {X : Type u} (TX: Set (Set X)) (hTX : IsTopology TX) (x : X) :
-  net_converges TX (neighborhood_net TX hTX x) x := by
+def neighborhood_net (T: Set (Set X)) (x: X): Endorelation (Nbhds T x) :=
+  fun ⟨U, _⟩ ⟨V, _⟩ => V ⊆ U
+
+theorem neighborhood_net_directed {T: Set (Set X)} (hT: IsTopology T) (x: X) :
+  directed (neighborhood_net T x) := {
+  reflexive := fun U => Set.Subset.refl U.1,
+  transitive := by exact fun _ _ _ h1 h2 _ h3 ↦ h1 (h2 h3)
+  upperbound := fun U V => by
+    have h_inter_nhds: U.1 ∩ V.1 ∈ Nbhds T x := by
+      obtain ⟨O_U, hO_U_open, hx_in_OU, hOU_sub_U⟩ := U.2
+      obtain ⟨O_V, hO_V_open, hx_in_OV, hOV_sub_V⟩ := V.2
+      use O_U ∩ O_V
+      exact ⟨binary_inter_open hT hO_U_open hO_V_open, ⟨hx_in_OU, hx_in_OV⟩, Set.inter_subset_inter hOU_sub_U hOV_sub_V⟩
+    use ⟨U.1 ∩ V.1, h_inter_nhds⟩
+    exact ⟨Set.inter_subset_left, Set.inter_subset_right⟩
+}
+
+theorem neighborhood_net_converges {T: Set (Set X)} (hT: IsTopology T) (x: X) :
+  net_converges T (neighborhood_net T x) (fun _ => x) x := by
   rw [net_converges]
-  intro U hU_open hx_in_U
-  use ⟨U, open_neighborhood TX hx_in_U hU_open⟩
-  rintro ⟨A, hA⟩ hA_sub_U
-  have point_in_A := Classical.choose_spec (Set.nonempty_of_mem (neighborhood_mem hA))
-  exact hA_sub_U point_in_A
+  intro _ hU
+  exists ⟨Set.univ, neighborhood_univ hT x⟩
+  intros
+  exact neighborhood_mem hU
 
-
-
-
-theorem continuous_at_iff_f_net_converges
-  {X Y : Type*} (TX: Set (Set X))(TY: Set (Set Y))
-  (hTX : IsTopology TX) (hTY : IsTopology TY)
-  (f : X → Y) (x0 : X) :
-  continuous_at TX TY f x0 ↔
-    ∀ n : net X, net_converges TX n x0 → f_net_converges TY f n (f x0):= by
-    constructor
-    intro h n hn
-    rw[continuous_at] at h
-    simp[f_net_converges,net_converges]
-    intro U hU hf
-    have h1 : U∈ Nbhds TY (f x0) := by
-      simp [Nbhds]
-      exact open_neighborhood TY hf hU
-    apply h at h1
-    obtain ⟨ N,hN⟩ := h1
-    simp [f_net]
-    simp[net_converges] at hn
-    simp [Nbhds,neighborhood] at hN
-    obtain ⟨ O,hO⟩ := hN.left
-    let h3:= hO.left
-    apply hn at h3
-    have h4: x0∈ O:= by exact hO.right.left
-    apply h3 at h4
-    obtain ⟨ i,hi⟩ := h4
-    use i
-    intro j hj
-    exact hN.2 (hO.2.2 (hi j hj))
-    intro hn N hN
+theorem continuous_at_iff_all_nets_converge {X: Type u} {Y: Type v} {TX: Set (Set X)} {TY: Set (Set Y)}
+  (hTX: IsTopology TX) (hTY: IsTopology TY) (f: X → Y) (x0: X):
+  continuous_at TX TY f x0 ↔ ∀ D: Type v, ∀ R: Endorelation D, ∀ x: D → X,
+    directed R → net_converges TX R x x0 → net_converges TY R (f ∘ x) (f x0) := by
+  constructor
+  · intro hf D R x h1 h2 V hV
+    obtain ⟨U, hU1, hU2⟩ := hf V hV
+    obtain ⟨i₀, hi₀⟩ := h2 U hU1
+    exists i₀
+    intro i hi
+    simp_all
+    exact hU2 (hi₀ i hi)
+  · intro h
+    have := h (Nbhds TY (f x0)) (neighborhood_net TY (f x0))
+    -- take D = Nbhds(x)?
     sorry
